put state calculus stuff into separate file

src/FlattenExpr.v
@@ -5,6 +5,7 @@ Require compiler.ExprImp.
 Require compiler.FlatImp.
 Require Import Coq.Logic.FunctionalExtensionality.
 Require Import compiler.Axioms.
+Require Import compiler.StateCalculus.
 
 Section FlattenExpr.
 
@@ -95,26 +96,6 @@ Section FlattenExpr.
     end.
   *)
 
-  Definition extends(s1 s2: state) := forall x v, get s2 x = Some v -> get s1 x = Some v.
-
-  Lemma extends_refl: forall s, extends s s.
-  Proof. unfold extends. firstorder. Qed.
-
-  Lemma put_extends: forall s x v,
-    extends (put s x v) s.
-  Proof. unfold extends. intros. Abort.
-
-  (* models a set of vars *)
-  Definition vars := var -> Prop.
-
-  Definition vars_empty: vars := fun _ => False.
-
-  Definition vars_one(x: var): vars := fun y => x = y.
-
-  Definition vars_union(vs1 vs2: vars): vars := fun x => vs1 x \/ vs2 x.
-
-  Definition vars_add(vs: vars)(new: var): vars := vars_union vs (vars_one new).
-
   (* returns the set of modified vars *)
   Fixpoint modVars(s: @FlatImp.stmt w): vars :=
     match s with
@@ -129,45 +110,6 @@ Section FlattenExpr.
         vars_union (modVars s1) (modVars s2)
     | FlatImp.SSkip => vars_empty
     end.
-
-  Definition only_differ(s1: state)(vs: vars)(s2: state) :=
-    forall x, vs x \/ get s1 x = get s2 x.
-
-  Lemma only_differ_union_l: forall s1 s2 r1 r2,
-    only_differ s1 r1 s2 ->
-    only_differ s1 (vars_union r1 r2) s2.
-  Proof. firstorder. Qed.
-
-  Lemma only_differ_union_r: forall s1 s2 r1 r2,
-    only_differ s1 r2 s2 ->
-    only_differ s1 (vars_union r1 r2) s2.
-  Proof. firstorder. Qed.
-
-  Lemma only_differ_one: forall s x v,
-    only_differ s (vars_one x) (put s x v).
-  Proof.
-    cbv [only_differ vars_one]. intros. destruct (dec (x = x0)); [ auto | ].
-    right. symmetry. apply get_put_diff. assumption.
-  Qed.
-
-  Lemma only_differ_refl: forall s1 r,
-    only_differ s1 r s1.
-  Proof. firstorder. Qed.
-
-  Lemma only_differ_sym: forall s1 s2 r,
-    only_differ s1 r s2 ->
-    only_differ s2 r s1.
-  Proof. firstorder. Qed.
-
-  Lemma only_differ_trans: forall s1 s2 s3 r,
-    only_differ s1 r s2 ->
-    only_differ s2 r s3 ->
-    only_differ s1 r s3.
-  Proof.
-    unfold only_differ. introv E1 E2. intro x.
-    specialize (E1 x). specialize (E2 x).
-    destruct E1; [auto|]. destruct E2; [auto|]. right. congruence.
-  Qed.
 
   Lemma invert_eval_SLoop: forall fuel st1 body1 cond body2 st4,
     FlatImp.eval_stmt (S fuel) st1 (FlatImp.SLoop body1 cond body2) = Success st4 ->
@@ -349,83 +291,12 @@ Section FlattenExpr.
      + simpl. inversionss. reflexivity.
   Qed.
 
-  Definition undef(s: state)(vs: vars) := forall x, vs x -> get s x = None.
-
-  Definition subset(vs1 vs2: vars) := forall x, vs1 x -> vs2 x.
-
   Definition vars_range_subset: forall lo1 hi1 lo2 hi2,
     lo1 >= lo2 ->
     hi1 <= hi2 ->
     subset (vars_range lo1 hi1) (vars_range lo2 hi2).
   Proof.
     unfold subset, vars_range. intros. omega.
-  Qed.
-
-  Lemma undef_shrink: forall st vs1 vs2,
-    undef st vs1 ->
-    subset vs2 vs1 ->
-    undef st vs2.
-  Proof. unfold undef, subset. firstorder. Qed.
-
-  Lemma only_differ_subset: forall s1 s2 r1 r2,
-    subset r1 r2 ->
-    only_differ s1 r1 s2 ->
-    only_differ s1 r2 s2.
-  Proof.
-    unfold subset, only_differ. intros. firstorder.
-  Qed.
-
-  Lemma extends_if_only_differ_in_undef: forall s1 s2 s vs,
-    extends s1 s ->
-    undef s vs ->
-    only_differ s1 vs s2 ->
-    extends s2 s.
-  Proof.
-    unfold extends, undef, only_differ.
-    introv E U O G.
-    specialize (O x). destruct O as [O | O].
-    - specialize (U _ O). congruence. (* contradiction *)
-    - rewrite <- O. apply E. assumption.
-  Qed.
-
-  Lemma extends_if_only_differ_is_undef: forall s1 s2 vs,
-    undef s1 vs ->
-    only_differ s1 vs s2 ->
-    extends s2 s1.
-  Proof.
-    intros. eapply extends_if_only_differ_in_undef; [eapply extends_refl | eassumption..].
-  Qed.
-
-  Lemma extends_put_same: forall s1 s2 x v,
-    extends s2 s1 ->
-    extends (put s2 x v) (put s1 x v).
-  Proof.
-    unfold extends. introv E G.
-    destruct (dec (x = x0)).
-    - subst x0. rewrite get_put_same in G. inversion G. subst v0; clear G.
-      apply get_put_same.
-    - rewrite get_put_diff by assumption.
-      rewrite get_put_diff in G by assumption. auto.
-  Qed.
-
-  Lemma only_differ_get_unchanged: forall s1 s2 x v d,
-    get s1 x = v ->
-    only_differ s1 d s2 ->
-    ~ d x ->
-    get s2 x = v.
-  Proof.
-    introv G D N.
-    unfold only_differ in D. destruct (D x); congruence.
-  Qed.
-
-  Lemma only_differ_put: forall s (d: vars) x v,
-    d x ->
-    only_differ s d (put s x v).
-  Proof.
-    unfold only_differ. intros.
-    destruct (dec (x = x0)).
-    - subst x0. left. assumption.
-    - right. rewrite get_put_diff; auto.
   Qed.
 
   Lemma flattenExpr_correct_aux: forall e firstFree resVar s initialH initialL res,
@@ -487,7 +358,7 @@ Section FlattenExpr.
         }
         rewrite G1'. simpl. rewrite G2. simpl. reflexivity.
       + apply get_put_same.
-      + apply only_differ_trans with (s2 := midL).
+      + rename s1 into stat1. apply only_differ_trans with (s2 := midL).
         * eapply only_differ_subset; [|eassumption].
           repeat match goal with
           | H : _  |- _ => apply flattenExpr_modVars_spec in H
@@ -570,6 +441,6 @@ Section FlattenExpr.
         * admit. (* TODO only_differ *)
       +
 
-  Qed.
+  Abort.
 
 End FlattenExpr.
