src/StateCalculus.v
@@ -1,0 +1,144 @@
+Require Import lib.LibTactics.
+Require Import Coq.Logic.FunctionalExtensionality.
+Require Import compiler.Axioms.
+Require Import compiler.Common.
+
+Section StateCalculus.
+
+  Context {var: Type}. (* variable name (key) *)
+  Context {dec_eq_var: DecidableEq var}.
+  Context {val: Type}. (* value *)
+  Context {state: Type}.
+  Context {stateMap: compiler.Common.Map state var val}.
+
+  Definition extends(s1 s2: state) := forall x v, get s2 x = Some v -> get s1 x = Some v.
+
+  Lemma extends_refl: forall s, extends s s.
+  Proof. unfold extends. firstorder. Qed.
+
+  Lemma put_extends: forall s x v,
+    extends (put s x v) s.
+  Proof. unfold extends. intros. Abort.
+
+  (* models a set of vars *)
+  Definition vars := var -> Prop.
+
+  Definition vars_empty: vars := fun _ => False.
+
+  Definition vars_one(x: var): vars := fun y => x = y.
+
+  Definition vars_union(vs1 vs2: vars): vars := fun x => vs1 x \/ vs2 x.
+
+  Definition vars_add(vs: vars)(new: var): vars := vars_union vs (vars_one new).
+
+  Definition only_differ(s1: state)(vs: vars)(s2: state) :=
+    forall x, vs x \/ get s1 x = get s2 x.
+
+  Lemma only_differ_union_l: forall s1 s2 r1 r2,
+    only_differ s1 r1 s2 ->
+    only_differ s1 (vars_union r1 r2) s2.
+  Proof. firstorder. Qed.
+
+  Lemma only_differ_union_r: forall s1 s2 r1 r2,
+    only_differ s1 r2 s2 ->
+    only_differ s1 (vars_union r1 r2) s2.
+  Proof. firstorder. Qed.
+
+  Lemma only_differ_one: forall s x v,
+    only_differ s (vars_one x) (put s x v).
+  Proof.
+    cbv [only_differ vars_one]. intros. destruct (dec (x = x0)); [ auto | ].
+    right. symmetry. apply get_put_diff. assumption.
+  Qed.
+
+  Lemma only_differ_refl: forall s1 r,
+    only_differ s1 r s1.
+  Proof. firstorder. Qed.
+
+  Lemma only_differ_sym: forall s1 s2 r,
+    only_differ s1 r s2 ->
+    only_differ s2 r s1.
+  Proof. firstorder. Qed.
+
+  Lemma only_differ_trans: forall s1 s2 s3 r,
+    only_differ s1 r s2 ->
+    only_differ s2 r s3 ->
+    only_differ s1 r s3.
+  Proof.
+    unfold only_differ. introv E1 E2. intro x.
+    specialize (E1 x). specialize (E2 x).
+    destruct E1; [auto|]. destruct E2; [auto|]. right. congruence.
+  Qed.
+
+  Definition undef(s: state)(vs: vars) := forall x, vs x -> get s x = None.
+
+  Definition subset(vs1 vs2: vars) := forall x, vs1 x -> vs2 x.
+
+  Lemma undef_shrink: forall st vs1 vs2,
+    undef st vs1 ->
+    subset vs2 vs1 ->
+    undef st vs2.
+  Proof. unfold undef, subset. firstorder. Qed.
+
+  Lemma only_differ_subset: forall s1 s2 r1 r2,
+    subset r1 r2 ->
+    only_differ s1 r1 s2 ->
+    only_differ s1 r2 s2.
+  Proof.
+    unfold subset, only_differ. intros. firstorder.
+  Qed.
+
+  Lemma extends_if_only_differ_in_undef: forall s1 s2 s vs,
+    extends s1 s ->
+    undef s vs ->
+    only_differ s1 vs s2 ->
+    extends s2 s.
+  Proof.
+    unfold extends, undef, only_differ.
+    introv E U O G.
+    specialize (O x). destruct O as [O | O].
+    - specialize (U _ O). congruence. (* contradiction *)
+    - rewrite <- O. apply E. assumption.
+  Qed.
+
+  Lemma extends_if_only_differ_is_undef: forall s1 s2 vs,
+    undef s1 vs ->
+    only_differ s1 vs s2 ->
+    extends s2 s1.
+  Proof.
+    intros. eapply extends_if_only_differ_in_undef; [eapply extends_refl | eassumption..].
+  Qed.
+
+  Lemma extends_put_same: forall s1 s2 x v,
+    extends s2 s1 ->
+    extends (put s2 x v) (put s1 x v).
+  Proof.
+    unfold extends. introv E G.
+    destruct (dec (x = x0)).
+    - subst x0. rewrite get_put_same in G. inversion G. subst v0; clear G.
+      apply get_put_same.
+    - rewrite get_put_diff by assumption.
+      rewrite get_put_diff in G by assumption. auto.
+  Qed.
+
+  Lemma only_differ_get_unchanged: forall s1 s2 x v d,
+    get s1 x = v ->
+    only_differ s1 d s2 ->
+    ~ d x ->
+    get s2 x = v.
+  Proof.
+    introv G D N.
+    unfold only_differ in D. destruct (D x); congruence.
+  Qed.
+
+  Lemma only_differ_put: forall s (d: vars) x v,
+    d x ->
+    only_differ s d (put s x v).
+  Proof.
+    unfold only_differ. intros.
+    destruct (dec (x = x0)).
+    - subst x0. left. assumption.
+    - right. rewrite get_put_diff; auto.
+  Qed.
+
+End StateCalculus.
